Function extensionality

Gt3/JEq/Basic.lean
@@ -99,12 +99,16 @@ inductive Ctx.JEq : Ctx → Tm 0 → Tm 0 → Tm 0 → Prop
     (rhs_wf : JEq Γ Ba ba ba)
     (hba : JEq Γ Ba (b.lst a) ba)
     : JEq Γ Ba (.app (A.abs b) a) ba
-  | beta_fst' {Γ}  {A : Tm 0} {B : Tm 1} {a b : Tm 0}
+  | beta_fst' {Γ}  {A : Tm 0} {B : Tm 1} {a b : Tm 0} {m n} {L : Finset String}
+    (hA : JEq Γ (.univ m) A A)
+    (hB : ∀ x ∉ L, JEq (Γ.cons x A) (.univ n) (B.open x) (B.open x))
     (hp : JEq Γ (.sigma A B) (.pair a b) (.pair a b))
     (lhs_wf : JEq Γ A (.fst (.pair a b)) (.fst (.pair a b)))
     (rhs_wf : JEq Γ A a a)
     : JEq Γ A (.fst (.pair a b)) a
-  | beta_snd' {Γ}  {A : Tm 0} {B : Tm 1} {a b Ba : Tm 0}
+  | beta_snd' {Γ}  {A : Tm 0} {B : Tm 1} {a b Ba : Tm 0} {m n} {L : Finset String}
+    (hA : JEq Γ (.univ m) A A)
+    (hB : ∀ x ∉ L, JEq (Γ.cons x A) (.univ n) (B.open x) (B.open x))
     (hp : JEq Γ (.sigma A B) (.pair a b) (.pair a b))
     (lhs_wf : JEq Γ Ba (.snd (.pair a b)) (.snd (.pair a b)))
     (rhs_wf : JEq Γ Ba b b)
@@ -152,6 +156,13 @@ inductive Ctx.JEq : Ctx → Tm 0 → Tm 0 → Tm 0 → Prop
     (rhs_wf : JEq Γ (.univ 0) .unit .unit)
     : JEq Γ (.univ 0) φc .unit
   -- Reflexivity and extensionality
+  | funext' {Γ} {A : Tm 0} {B : Tm 1} {f g : Tm 0} {m n} {L : Finset String}
+    (hA : JEq Γ (.univ m) A A)
+    (hB : ∀ x ∉ L, JEq (Γ.cons x A) (.univ n) (B.open x) (B.open x))
+    (hf : JEq Γ (A.pi B) f f)
+    (hg : JEq Γ (A.pi B) g g)
+    (hfg : ∀x ∉ L, JEq (Γ.cons x A) (B.open x) (f.app (.fv x)) (g.app (.fv x)))
+    : JEq Γ (A.pi B) f g
   | eqn_rfl {Γ} {A a b: Tm 0} : JEq Γ A a b → JEq Γ (.univ 0) (.eqn a b) .unit
   | eqn_ext {Γ} {A a b : Tm 0}
     : JEq Γ A a a → JEq Γ A b b → JEq Γ (.univ 0) (.eqn a b) .unit → JEq Γ A a b
